lemmas

examples/refinement/layering/LowStar.Lens.DependentMap.fst
@@ -5,7 +5,10 @@ open FStar.HyperStack.ST
 open FStar.Tactics
 open FStar.BigOps
 open FStar.Classical 
+open LowStar.BufferOps 
+open FStar.Modifies
 
+module L = LowStar.Lens
 module DGM = FStar.DependentGMap
 module DM = FStar.DependentMap
 
@@ -14,25 +17,20 @@ module HS = FStar.HyperStack
 module HST = FStar.HyperStack.ST
 module LB = LowStar.Lens.Buffer
 module List = FStar.List.Tot.Base
+module ListP = FStar.List.Tot.Properties
 
-// DependentMap iterators on the sub-domain of interest
-
-// let fold (#t:eqtype) #a (f:t -> Type) (m:DM.t t f) (dom:list t) 
-//   (h : (k:t -> b:(f k) -> a -> a)) (acc : a) : GTot a = 
-//   List.fold_left (fun v k -> h k (DM.sel m k) v) acc dom 
-
-// let map  (#t:eqtype) #a (f:t -> Type) (m:DM.t t f) (dom:list t) 
-//   (h : (k:t -> b:(f k) -> a)) : list a = 
-//   List.map (fun k -> h k (DM.sel m k)) dom 
-
-// // List of dependent pairs from a dependent map
-// let to_list (#t:eqtype) (f:t -> Type) (m:DM.t t f) (dom:list t) : list (x:t & (f x)) = 
-//   List.map (fun k -> (| k,  DM.sel m k |)) dom 
+unfold 
+let fin (#a:eqtype) (lst:list a) = (forall x. List.memP x lst) /\ List.noRepeats lst
 
 // all pointers in a heap are live in a given mem 
 unfold
-let map_inv (#t:eqtype) (f: t -> Type) (m:DM.t t (fun (x:t) -> B.pointer (f x))) (dom:list t) (h : HS.mem) : Type0 =
+let map_inv' (#t:eqtype) (f: t -> Type) (m:DM.t t (fun (x:t) -> B.pointer (f x))) (dom:list t) (h : HS.mem) : Type0 =
   big_and' #t (fun x -> B.live h (DM.sel m x)) dom
+
+unfold 
+let map_inv (#t:eqtype) (f: t -> Type) (m:DM.t t (fun (x:t) -> B.pointer (f x))) (h : HS.mem) : Type0 =
+  forall (x:t). B.live h (DM.sel m x)
+  
 
 // locations of a dependent map
 let rec map_loc (#t:eqtype) (f: t -> Type) (m:DM.t t (fun (x:t) -> B.pointer (f x))) (dom:list t) : GTot B.loc =
@@ -44,9 +42,12 @@ match dom with
 let map_eloc #t f m dom : eloc = Ghost.hide (map_loc #t f m dom)
 
 // Lemmas about map_inv
-let map_inv_mem (#t:eqtype) (f: t -> Type) (m:DM.t t (fun (x:t) -> B.pointer (f x)))
-   (dom:list t) (h : imem (map_inv f m dom)) (x:t{List.memP x dom}) : Lemma (B.live h (DM.sel m x)) =
+let map_inv_mem' (#t:eqtype) (f: t -> Type) (m:DM.t t (fun (x:t) -> B.pointer (f x)))
+   (dom:list t) (h : imem (map_inv' f m dom)) (x:t{List.memP x dom}) : Lemma (B.live h (DM.sel m x)) =
    let p = big_and'_forall #t (fun x -> B.live h (DM.sel m x)) dom in ()
+
+let map_inv_mem (#t:eqtype) (f: t -> Type) (m:DM.t t (fun (x:t) -> B.pointer (f x)))
+  (h : imem (map_inv f m)) (x:t) : Lemma (B.live h (DM.sel m x)) = ()
 
 (* Preservation of liveness after memory updates *)
 
@@ -55,20 +56,19 @@ val g_upd_preserves_live : #a:Type -> #b:Type -> h:HS.mem -> b1:B.pointer a{B.li
                                    
 let g_upd_preserves_live #a #b h b1 b2 v = 
   let p = B.g_upd_seq_as_seq b1 (Seq.upd (B.as_seq h b1) 0 v) h in ()
+  
+// update preserves livenes of the pointer being updated and the heap invariant
+val g_upd_preserves_map_inv' : #a:Type -> #t:eqtype -> f:(t -> Type) -> h:HS.mem -> b:B.pointer a{B.live h b} -> v:a ->
+  ptr:(DM.t t (fun (x:t) -> B.pointer (f x))) -> dom:list t{map_inv' f ptr dom h} ->
+  Lemma (let h' = B.g_upd b 0 v h in B.modifies (B.loc_buffer b) h h' /\ B.live h' b /\ map_inv' f ptr dom h')
 
-// and update preserves livenes of the pointer being updated and of any other live list in the heap  
-val g_upd_preserves_map_inv : #a:Type -> #t:eqtype -> f:(t -> Type) -> h:HS.mem -> b:B.pointer a{B.live h b} -> v:a ->
-  ptr:(DM.t t (fun (x:t) -> B.pointer (f x))) -> dom:list t{map_inv f ptr dom h} ->
-  Lemma (let h' = B.g_upd b 0 v h in B.modifies (B.loc_buffer b) h h' /\ B.live h' b /\ map_inv f ptr dom h')
-
-
-let g_upd_preserves_map_inv #a #t f h b v ptr dom = 
+let g_upd_preserves_map_inv' #a #t f h b v ptr dom = 
   let h' = B.g_upd b 0 v h in
   let _ = g_upd_preserves_live h b b v in
   assert (B.live h' b);
   assert (B.modifies (B.loc_buffer b) h h');  
   // map liveness, going through all of the key   
-  let rec aux (ks : list t{map_inv f ptr ks h}) : Lemma (map_inv f ptr ks h') = 
+  let rec aux (ks : list t{map_inv' f ptr ks h}) : Lemma (map_inv' f ptr ks h') = 
     match ks with 
     | [] -> admit ()
     | k :: ks' -> 
@@ -77,24 +77,152 @@ let g_upd_preserves_map_inv #a #t f h b v ptr dom =
       assert (B.live h' b); 
       aux ks'
   in aux dom
-    
 
-unfold
-let dom (#a:eqtype) (lst:list a) : Tot eqtype = x:a{List.memP x lst} 
 
-unfold 
-let fin (#a:eqtype) (lst:list a) = (forall x. List.memP x lst) /\ List.noRepeats lst
+val g_upd_preserves_map_inv : #a:Type -> #t:eqtype -> f:(t -> Type) -> h:HS.mem -> b:B.pointer a{B.live h b} -> v:a ->
+  ptr:(DM.t t (fun (x:t) -> B.pointer (f x))){map_inv f ptr h} ->
+  Lemma (let h' = B.g_upd b 0 v h in B.modifies (B.loc_buffer b) h h' /\ B.live h' b /\ map_inv f ptr h')
+
+let g_upd_preserves_map_inv #a #t f h b v ptr =
+  let h' = B.g_upd b 0 v h in
+  let _ = g_upd_preserves_live h b b v in
+  assert (B.live h' b);
+  assert (B.modifies (B.loc_buffer b) h h'); 
+  let lem (x : t) : Lemma (B.live h' (DM.sel ptr x)) = 
+    let b' = DM.sel ptr x in
+    let h' = B.g_upd b 0 v h in
+    let _ = g_upd_preserves_live h b b' v in ()
+  in 
+  ()
+
+// Lemmas about map_eloc
+let map_loc_includes (#t:eqtype) (f: t -> Type) (m:DM.t t (fun (x:t) -> B.pointer (f x))) (dom:list t{fin dom}) (x:t) 
+: Lemma (B.loc_includes (map_loc f m dom) (B.loc_buffer (DM.sel m x))) = 
+  assert (List.memP x dom);
+  let rec aux (ks : list t {List.memP x ks}) : Lemma (ensures (B.loc_includes (map_loc f m ks) (B.loc_buffer (DM.sel m x)))) (decreases ks) =
+    match ks with 
+    | [] -> ()
+    | k :: ks' ->
+      if (x = k) then  
+        (B.loc_includes_refl (B.loc_buffer (DM.sel m k));
+         B.loc_includes_union_l (B.loc_buffer (DM.sel m x)) (map_loc f m ks') (B.loc_buffer (DM.sel m k)))
+      else 
+        (aux ks';
+         B.loc_includes_union_l (B.loc_buffer (DM.sel m k)) (map_loc f m ks') (B.loc_buffer (DM.sel m x)))
+  in aux dom
+
+let map_eloc_includes (#t:eqtype) (f: t -> Type) (m:DM.t t (fun (x:t) -> B.pointer (f x))) (dom:list t{fin dom}) x
+: Lemma (B.loc_includes (L.as_loc (map_eloc f m dom)) (B.loc_buffer (DM.sel m x))) =
+  map_loc_includes f m dom x 
+  
+let map_eloc_eq (#t:eqtype) (f: t -> Type) (m:DM.t t (fun (x:t) -> B.pointer (f x))) (ks:list t) 
+: Lemma (as_loc (map_eloc f m ks) == map_loc f m ks) = 
+  Ghost.reveal_hide (map_loc f m ks)
+
+
+(** put *)
+let rec put_aux (#t:eqtype) (f:t -> Type) (keys:list t) (ptr:DM.t t (fun x -> B.pointer (f x))) (vmap : DGM.t t f) (h : imem (map_inv f ptr))
+: GTot (imem (map_inv f ptr)) =
+  match keys with 
+  | [] -> h 
+  | k :: ks' -> 
+    let b = DM.sel ptr k in 
+    let v = DGM.sel vmap k in 
+    let h' = B.g_upd b 0 v h in
+    (* liveness preservation *)
+     let _ = g_upd_preserves_map_inv f h b v ptr in 
+     put_aux f ks' ptr vmap h'
+
+let put (#t:eqtype) (f:t -> Type) (keys:list t) (ptr:DM.t t (fun x -> B.pointer (f x))) : put_t (imem (map_inv f ptr)) (DGM.t t f) = put_aux f keys ptr 
+
+(** get *) 
+let get (#t:eqtype) (f:t -> Type) (ptr:DM.t t (fun x -> B.pointer (f x))) : get_t (imem (map_inv f ptr)) (DGM.t t f) = 
+  let aux h = 
+    let value (k:t) : GTot (f k) =
+      let b = DM.sel ptr k in 
+      let _ = map_inv_mem #t f ptr h k in 
+      assert (B.live h b);
+      B.get h b 0
+    in DGM.create value in aux
+
+
+let get_eq (#t:eqtype) (f:t -> Type) (ptr:DM.t t (fun x -> B.pointer (f x))) (x:t) (h : (imem (map_inv f ptr)))
+: Lemma (DGM.sel (get f ptr h) x == (let b = DM.sel ptr x in 
+                                     let _ = map_inv_mem #t f ptr h x in 
+                                     B.get h b 0)) = ()
+
+
+
+
+let put_modifies_lemma' (#t:eqtype) (f:t -> Type) (keys:list t{fin keys}) (ptr:DM.t t (fun x -> B.pointer (f x))) (vmap : DGM.t t f) (h : imem (map_inv f ptr))
+: Lemma (B.modifies (as_loc (map_eloc f ptr keys)) h (put f keys ptr vmap h))[SMTPat (put f keys ptr vmap h)]  = 
+let rec aux (ks : list t) (h : imem (map_inv f ptr)) : Lemma (B.modifies (as_loc (map_eloc f ptr ks)) h (put f ks ptr vmap h)) = 
+   match ks with 
+   | [] -> B.modifies_refl (as_loc (map_eloc f ptr ks)) h
+   | k :: ks' ->
+     let b = DM.sel ptr k in 
+     let v = DGM.sel vmap k in 
+     let h' = B.g_upd b 0 v h in
+     let _ = g_upd_preserves_map_inv f h b v ptr in 
+     aux ks' h';
+     B.modifies_trans (B.loc_buffer b) h h' (as_loc (map_eloc f ptr ks')) (put f ks' ptr vmap h');
+     map_eloc_eq f ptr ks';
+     map_eloc_eq f ptr ks;
+     assert (B.modifies (as_loc (map_eloc f ptr ks)) h (put f ks ptr vmap h))
+ in aux keys h
+
+ let put_modifies_lemma (#t:eqtype) (f:t -> Type) (keys:list t{fin keys}) (ptr:DM.t t (fun x -> B.pointer (f x)))
+ : Lemma (put_modifies_loc #_ #(map_inv f ptr) (map_eloc f ptr keys) (put f keys ptr)) =  
+ let _ = put_modifies_lemma' f keys ptr in ()
+  
+
+(* First lens law *)
+let put_property (#t:eqtype) (f:t -> Type) (keys:list t{fin keys}) (ptr:DM.t t (fun x -> B.pointer (f x)))
+  (m : DGM.t t f) (h : (imem (map_inv f ptr))) (k : t) : Lemma (let b = DM.sel ptr k in B.get (put f keys ptr m h) b 0 == DGM.sel m k) =
+  admit ()
+
+
+let get_put_lem (#t:eqtype) (f:t -> Type) (keys:list t{fin keys}) (ptr:DM.t t (fun x -> B.pointer (f x))) 
+  (h : (imem (map_inv f ptr))) (m : DGM.t t f) (k : t) : Lemma (DGM.sel (get f keys ptr (put f keys ptr m h)) k == DGM.sel m k) = 
+   let h' = put f keys ptr m h in 
+   let _ = put_property f keys ptr m h k in  // main assumption about put
+   () 
+   
+   
+let get_put_lem_ext (#t:eqtype) (f:t -> Type) (keys:list t{fin keys}) (ptr:DM.t t (fun x -> B.pointer (f x))) 
+  (h : (imem (map_inv f ptr))) (m : DGM.t t f) : Lemma (get f keys ptr (put f keys ptr m h) == m)[SMTPat (get f keys ptr (put f keys ptr m h))] = 
+  forall_intro (get_put_lem f keys ptr h m);
+  DGM.equal_elim (get  f keys ptr (put  f keys ptr m h)) m
+
+// These do not work when nested 
+let get_put_law (#t:eqtype) (f:t -> Type) (keys:list t{fin keys}) (ptr:DM.t t (fun x -> B.pointer (f x))) : Lemma (get_put (get f keys ptr) (put f keys ptr)) = 
+  let p = get_put_lem_ext f keys ptr in
+  ()
+
+let get_put_law' (#t:eqtype) (f:t -> Type) (keys:list t{fin keys}) (ptr:DM.t t (fun x -> B.pointer (f x))) : squash (get_put (get f keys ptr) (put f keys ptr)) = 
+  let p = get_put_lem_ext f keys ptr in
+  ()
+
+
+
+
+
+let mem_lens (#t:eqtype) (f:t -> Type) (keys:list t{fin keys}) (ptr:DM.t t (fun x -> B.pointer (f x))) fp : imem_lens (map_inv f ptr) (DGM.t t f) fp = { 
+  get = get f keys ptr;
+  put = put f keys ptr;
+  lens_laws = get_put_law' f keys ptr
+} 
 
 (* put helper *)
 
-// let rec put_aux (#t:eqtype) (f:t -> Type) (keys:list t{fin keys}) (ptr:DM.t t (fun x -> B.pointer (f x))) (vmap : DM.t t f) (h : imem (map_inv f ptr keys)) : GTot (imem (map_inv f ptr keys))  = 
+// let rec put_aux (#t:eqtype) (f:t -> Type) (keys:list t{fin keys}) (ptr:DGM.t t (fun x -> B.pointer (f x))) (vmap : DGM.t t f) (h : imem (map_inv f ptr keys)) : GTot (imem (map_inv f ptr keys))  = 
 //   let rec aux (ks : list t{List.noRepeats ks}) (h : imem (map_inv f ptr keys){map_inv f ptr ks h})
 //   : GTot (h':imem (map_inv f ptr keys){forall x, ~ List.mem x ks /\ B.live h x => B.get }) = 
 //     match ks with 
 //     | [] -> h 
 //     | k :: ks' ->
-//       let b = DM.sel ptr k in 
-//       let v = DM.sel vmap k in 
+//       let b = DGM.sel ptr k in 
+//       let v = DGM.sel vmap k in 
 //       let h' = B.g_upd b 0 v h in
 //       (* liveness preservation *)
 //       let _ = g_upd_preserves_map_inv f h b v ptr keys in 
@@ -103,14 +231,14 @@ let fin (#a:eqtype) (lst:list a) = (forall x. List.memP x lst) /\ List.noRepeats
 //   in aux keys h
 
 
-//   let rec put_aux (#t:eqtype) (f:t -> Type) (keys:list t{fin keys}) (ptr:DM.t t (fun x -> B.pointer (f x))) (vmap : DM.t t f) (h : imem (map_inv f ptr keys)) : GTot (imem (map_inv f ptr keys))  = 
+//   let rec put_aux (#t:eqtype) (f:t -> Type) (keys:list t{fin keys}) (ptr:DGM.t t (fun x -> B.pointer (f x))) (vmap : DGM.t t f) (h : imem (map_inv f ptr keys)) : GTot (imem (map_inv f ptr keys))  = 
 //     let rec aux (ks : list t{List.noRepeats ks}) (h : imem (map_inv f ptr keys){map_inv f ptr ks h})
 //     : GTot (h':imem (map_inv f ptr keys){ forall x}) = 
 //       match ks with 
 //       | [] -> h 
 //       | k :: ks' ->
-//         let b = DM.sel ptr k in 
-//         let v = DM.sel vmap k in 
+//         let b = DGM.sel ptr k in 
+//         let v = DGM.sel vmap k in 
 //         let h' = B.g_upd b 0 v h in
 //         (* liveness preservation *)
 //         let _ = g_upd_preserves_map_inv f h b v ptr keys in 
@@ -123,77 +251,49 @@ let fin (#a:eqtype) (lst:list a) = (forall x. List.memP x lst) /\ List.noRepeats
 
 (* Try 1 : every element of the type t is in the list *)
 
-let mk (#t:eqtype) (f:t -> Type) (keys:list t{fin keys}) (ptr:DM.t t (fun x -> B.pointer (f x))) (h:imem (map_inv f ptr keys)) 
-: hs_lens (DM.t t (fun (x:t) -> B.pointer (f x))) (DM.t t f) =
+let mk (#t:eqtype) (f:t -> Type) (keys:list t{fin keys}) (ptr:DM.t t (fun x -> B.pointer (f x))) (h:imem (map_inv f ptr)) 
+: hs_lens (DM.t t (fun (x:t) -> B.pointer (f x))) (DGM.t t f) =
   (* invariant *) 
-  let inv = map_inv f ptr keys in
+  let inv = map_inv f ptr in
   (* mem snapshot *)
-  let (snap : imem (map_inv f ptr keys)) = h in 
+  let (snap : imem (map_inv f ptr)) = h in 
   (* footprint *)
   let fp = map_eloc #t f ptr keys in
-  (* put *)
-  let put : put_t (imem (map_inv f ptr keys)) (DM.t t f) = 
-    let rec aux (ks : list t) (vmap : DM.t t f) (h : imem (map_inv f ptr keys){map_inv f ptr ks h})
-    : GTot (imem (map_inv f ptr keys))  = 
-      match ks with 
-      | [] -> h 
-      | k :: ks' ->
-        let b = DM.sel ptr k in 
-        let v = DM.sel vmap k in 
-        let h' = B.g_upd b 0 v h in
-        (* liveness preservation *)
-        let _ = g_upd_preserves_map_inv f h b v ptr keys in 
-        let _ = g_upd_preserves_map_inv f h b v ptr ks' in   
-        aux ks' vmap h'
-    in aux keys
-  in
-  (* get *) 
-  let get : get_t (imem (map_inv f ptr keys)) (DM.t t f) = 
-    let aux h = 
-      let value (k:t) : GTot (f k) =
-        let b = DM.sel ptr k in 
-        let _ = map_inv_mem #t f ptr keys h k in 
-        assert (B.live h b);
-        B.get h b 0
-      in DM.create value in aux
-  in 
-  (* First lens law *)
-  let put_property (m : DM.t t f) (h : (imem (map_inv f ptr keys))) (k : t) : Lemma (let b = DM.sel ptr k in B.get (put m h) b 0 == DM.sel m k) =
-    admit ()
-  in
-  let get_put_lem (h : (imem (map_inv f ptr keys))) (m : DM.t t f) (k : t) : Lemma (DM.sel (get (put m h)) k == DM.sel m k) = 
-     let h' = put m h in 
-     let _ = put_property m h k in  // main assumption about put
-     let value (k:t) : GTot (f k) =
-       let b = DM.sel ptr k in 
-       let _ = map_inv_mem #t f ptr keys h k in 
-       B.get h' b 0
-     in     
-     let _ = DM.sel_create value k in 
-     assert (DM.sel (get h') k == (let b = DM.sel ptr k in 
-                                   let _ = map_inv_mem #t f ptr keys h k in 
-                                   B.get h' b 0));
-     ()
-  in
-  let get_put_lem_ext (h : (imem (map_inv f ptr keys))) (m : DM.t t f) : Lemma (get (put m h) == m)[SMTPat (get (put m h))] = 
-      forall_intro (get_put_lem h m);
-      DM.equal_elim (get (put m h)) m
-  in
-  // let get_put' () : Lemma (get_put get put) =
-  //   forall_intro_2 #(imem (map_inv f ptr keys)) #(fun _ -> DM.t t f) #(fun h m -> get (put m h) == m) get_put_lem_ext in 
-  let l : imem_lens inv (DM.t t f) fp = { 
-    get = get;
-    put = put;
-    lens_laws = admit () // XXX
-  } in
   { 
     footprint = fp;
-    invariant = (fun ptr -> map_inv f ptr keys);
+    invariant = map_inv f;
     x = ptr;
     snapshot = snap;
     l = l
   }
+ 
+
+// Get and set 
   
+// read ith buffer
+let read_i (#t:eqtype) (#f: t -> Type) (l : hs_lens (DM.t t (fun (x:t) -> B.pointer (f x))) (DGM.t t f)) 
+      (i:t) : LensST (f i) l  // TODO : write field lens i 
+                  (requires (fun f1 -> True)) 
+                  (ensures (fun f1 v f2 -> f1 == f2 /\ v == DGM.sel f2 i)) = 
+  reveal_inv ();
+  let h = HST.get () in 
+  assert (L.inv l h);
+  assert (map_inv f l.x h);
+  let b = DM.sel l.x i in 
+  //assert (B.live h b);
+  admit ()
+  //!*b
+
+  // write ith buffer
+  let write_i (i:dom) (v : f_t i) : LensST unit lens 
+                                    (requires (fun f1 -> True)) 
+                                    (ensures (fun f1 _ f2 -> DM.upd f1 i v  == f2)) = 
+      let b = DM.sel lens.x i in 
+      b *= v
+
+
+
+
 // Allocation: scoped allocation
 // Experiment: swap with dep map 
 // Get/put with lens composition 
@@ -203,7 +303,10 @@ let test1 =
 
 (* Idea 2 : the domain of the map is resrticted in the elements of the list *)
 
+unfold
+let dom (#a:eqtype) (lst:list a) : Tot eqtype = x:a{List.memP x lst} 
+
 // let coerce (#a:eqtype) (l : list a) : list (dom #a l) = admit ()
 
-// let mk2 (#t:eqtype) (f:t -> Type) (keys:list t) (ptr:DM.t (dom keys) (fun x -> B.pointer (f x))) (h:imem (map_inv f ptr (coerce keys))) 
-// : hs_lens (DM.t (dom keys) (fun (x:t) -> B.pointer (f x))) (DM.t (dom keys) f) = admit ()
+// let mk2 (#t:eqtype) (f:t -> Type) (keys:list t) (ptr:DGM.t (dom keys) (fun x -> B.pointer (f x))) (h:imem (map_inv f ptr (coerce keys))) 
+// : hs_lens (DGM.t (dom keys) (fun (x:t) -> B.pointer (f x))) (DGM.t (dom keys) f) = admit ()
